feat: Nuon

Arithmetization/Exponential/Nuon.lean
@@ -12,65 +12,87 @@ variable {M : Type} [Zero M] [One M] [Add M] [Mul M] [LT M] [𝐏𝐀⁻.Mod M] 
 
 namespace Nuon
 
-@[simp] lemma llen_lt_len_hash_len (a : M) : ‖‖a‖‖ < ‖a # ‖a‖‖ := by
+@[simp] lemma llen_lt_len_hash_len (K : M) : ‖‖K‖‖ < ‖K # ‖K‖‖ := by
   simp [length_hash, lt_succ_iff_le]
-  rcases zero_le ‖a‖ with (ha | pos)
-  · simp [←ha]
+  rcases zero_le ‖K‖ with (hK | pos)
+  · simp [←hK]
   · exact le_mul_of_pos_left pos
 
-lemma mul_llen_lt_len_hash_len {i a : M} (hi : i ≤ ‖a‖) : i * ‖‖a‖‖ < ‖a # ‖a‖‖ := by
-  simp [length_hash, lt_succ_iff_le]; exact mul_le_mul_right' hi ‖‖a‖‖
+lemma mul_len_lt_len_hash {i I L : M} (hi : i ≤ ‖I‖) : i * ‖L‖ < ‖I # L‖ := by
+  simp [length_hash, lt_succ_iff_le]; exact mul_le_mul_right' hi ‖L‖
 
-def ext (a s i : M) : M := s / bexp (a # ‖a‖) (i * ‖‖a‖‖) % (‖a‖ # 1)
+lemma mul_len_lt_len_hash' {i K Z : M} (hi : i ≤ ‖z‖) : i * ‖‖K‖‖ < ‖z # ‖K‖‖ := by
+  simp [length_hash, lt_succ_iff_le]; exact mul_le_mul_right' hi ‖‖K‖‖
 
-lemma ext_add_of_dvd_sq_right {i s₁ s₂ p : M} (hi : i ≤ ‖a‖)
-    (pp : Pow2 p) (h : (i + 1) * ‖‖a‖‖ ≤ log p) :
-    ext a (s₁ + s₂ * p) i = ext a s₁ i := by
-  have : Exp ((i + 1) * ‖‖a‖‖) (bexp (a # ‖a‖) (i * ‖‖a‖‖) * ‖a‖ # 1) := by
+def ext (I L S i : M) : M := S / bexp (I # L) (i * ‖L‖) % (L # 1)
+
+local notation S "{" I ", " L "}[" i "]" => ext I L S i
+
+-- lemma ext_graph (I L S i y : M) : y = S{I, L}[i] ↔ ((‖I‖ < i ∨ ‖S‖ ≤ i * ‖L‖) ∧ y = 0) ∨ (∃ b ≤ S, Exp (i * ‖L‖) b ∧ y = S / b % (L # 1)) := by
+--   constructor
+--   · rintro rfl
+
+lemma ext_add_of_dvd_sq_right {I L i S₁ S₂ p : M} (hi : i ≤ ‖I‖)
+    (pp : Pow2 p) (h : (i + 1) * ‖L‖ ≤ log p) : (S₁ + S₂ * p){I, L}[i] = S₁{I, L}[i] := by
+  have : Exp ((i + 1) * ‖L‖) (bexp (I # L) (i * ‖L‖) * L # 1) := by
     simp [add_mul]
     exact Exp.add_mul
-      (by simp [mul_llen_lt_len_hash_len hi])
-      (by simpa using exp_hash ‖a‖ 1)
-  have : bexp (a # ‖a‖) (i * ‖‖a‖‖) * ‖a‖ # 1 ∣ p :=
-    Pow2.dvd_of_le (by simp; apply bexp_pow2; simp [mul_llen_lt_len_hash_len hi]) pp (this.monotone_le (exp_of_pow2 pp) h)
+      (by simp [mul_len_lt_len_hash hi])
+      (by simpa using exp_hash L 1)
+  have : bexp (I # L) (i * ‖L‖) * L # 1 ∣ p :=
+    Pow2.dvd_of_le (by simp; apply bexp_pow2; simp [mul_len_lt_len_hash hi]) pp (this.monotone_le (exp_of_pow2 pp) h)
   rcases this with ⟨p, rfl⟩
-  simp [ext, mul_comm s₂, mul_assoc]
-  have : 0 < bexp (a # ‖a‖) (i * ‖‖a‖‖) := bexp_pos (by simp [mul_llen_lt_len_hash_len hi])
+  simp [ext, mul_comm S₂, mul_assoc]
+  have : 0 < bexp (I # L) (i * ‖L‖) := bexp_pos (by simp [mul_len_lt_len_hash hi])
   simp [div_add_mul_self', this]
 
-def append (a s i x : M) : M := s % bexp (a # ‖a‖) (i * ‖‖a‖‖) + x * bexp (a # ‖a‖) (i * ‖‖a‖‖)
+def append (I L S i X : M) : M := S % bexp (I # L) (i * ‖L‖) + X * bexp (I # L) (i * ‖L‖)
 
-lemma append_lt_hash (s : M) {i x a} (hi : i ≤ ‖a‖) (hx : x ≤ ‖a‖) : append a s i x < 1 # ‖a‖ * a # ‖a‖ := calc
-  append a s i x < (x + 1) * bexp (a # ‖a‖) (i * ‖‖a‖‖)                := by simp [append, add_mul, add_comm]
-                                                                             exact mod_lt _ (bexp_pos $ mul_llen_lt_len_hash_len hi)
-  _              ≤ (‖a‖ + 1) * bexp (a # ‖a‖) (i * ‖‖a‖‖)              := mul_le_mul_right (by simp [hx])
-  _              ≤ bexp (a # ‖a‖) ‖‖a‖‖ * bexp (a # ‖a‖) (i * ‖‖a‖‖)   := mul_le_mul_right (by simp [succ_le_iff_lt]; apply lt_bexp_len (by simp))
-  _              ≤ bexp (a # ‖a‖) ‖‖a‖‖ * bexp (a # ‖a‖) (‖a‖ * ‖‖a‖‖) := mul_le_mul_left
-                                                                            ((bexp_monotone_le (mul_llen_lt_len_hash_len hi)
-                                                                              (mul_llen_lt_len_hash_len $ by rfl)).mpr (mul_le_mul_right hi))
-  _              = 1 # ‖a‖ * a # ‖a‖                                   := by congr 1
-                                                                             · exact bexp_eq_of_exp (by simp) (by simpa using exp_hash 1 ‖a‖)
-                                                                             · exact bexp_eq_of_exp (mul_llen_lt_len_hash_len $ by rfl) (exp_hash _ _)
+lemma append_lt_hash (S : M) {i X I L} (hi : i ≤ ‖I‖) (hx : X ≤ L) : append I L S i X < (L + 1) * I # L := calc
+  append I L S i X < (X + 1) * bexp (I # L) (i * ‖L‖)   := by simp [append, add_mul, add_comm]
+                                                              exact mod_lt _ (bexp_pos $ mul_len_lt_len_hash hi)
+  _                ≤ (L + 1) * bexp (I # L) (i * ‖L‖)   := mul_le_mul_right (by simp [hx])
+  _                ≤ (L + 1) * bexp (I # L) (‖I‖ * ‖L‖) := mul_le_mul_left ((bexp_monotone_le (mul_len_lt_len_hash hi) (by simp [length_hash])).mpr (mul_le_mul_right hi))
+  _                = (L + 1) * I # L                    := by congr 1; exact bexp_eq_of_exp (by simp [length_hash]) (exp_hash _ _)
 
-lemma ext_append_last (s : M) {i x a} (hi : i ≤ ‖a‖) (hx : x ≤ ‖a‖) : ext a (append a s i x) i = x := by
-  have he : Exp (i * ‖‖a‖‖) (bexp (a # ‖a‖) (i * ‖‖a‖‖)) := by simp [mul_llen_lt_len_hash_len hi]
-  have : x < ‖a‖ # 1 := lt_of_le_of_lt hx (by simp)
+lemma ext_append_last (S : M) {i X I L} (hi : i ≤ ‖I‖) (hx : X ≤ L) : (append I L S i X){I, L}[i] = X := by
+  have he : Exp (i * ‖L‖) (bexp (I # L) (i * ‖L‖)) := by simp [mul_len_lt_len_hash hi]
+  have : X < L # 1 := lt_of_le_of_lt hx (by simp)
   simp [ext, append, div_add_mul_self _ _ he.range_pos, this]
 
-lemma ext_append_last_lt (s : M) {i j x a} (hi : i ≤ ‖a‖) (hij : j < i) :
-    ext a (append a s i x) j = ext a s j :=
-  let q := bexp (a # ‖a‖) (i * ‖‖a‖‖)
-  have pq : Pow2 q := bexp_pow2 (by simp [mul_llen_lt_len_hash_len hi])
-  have hq : (j + 1) * ‖‖a‖‖ ≤ log q := by simp [log_bexp (mul_llen_lt_len_hash_len hi)]; exact mul_le_mul_right' (lt_iff_succ_le.mp hij) _
+lemma ext_append_lt (S : M) {i j X I L} (hi : i ≤ ‖I‖) (hij : j < i) :
+    (append I L S i X){I, L}[j] = S{I, L}[j] :=
+  let Q := bexp (I # L) (i * ‖L‖)
+  have pq : Pow2 Q := bexp_pow2 (by simp [mul_len_lt_len_hash hi])
+  have hq : (j + 1) * ‖L‖ ≤ log Q := by simp [log_bexp (mul_len_lt_len_hash hi)]; exact mul_le_mul_right' (lt_iff_succ_le.mp hij) _
   calc
-    ext a (append a s i x) j = ext a (s % q + x * q) j       := rfl
-    _                        = ext a (s % q) j               := ext_add_of_dvd_sq_right (le_trans (le_of_lt hij) hi) pq hq
-    _                        = ext a (s % q + (s / q) * q) j := Eq.symm <| ext_add_of_dvd_sq_right (le_trans (le_of_lt hij) hi) pq hq
-    _                        = ext a s j                     := by rw [mul_comm, add_comm, div_add_mod]
+    (append I L S i X){I, L}[j] = (S % Q + X * Q){I, L}[j]       := rfl
+    _                           = (S % Q){I, L}[j]               := ext_add_of_dvd_sq_right (le_trans (le_of_lt hij) hi) pq hq
+    _                           = (S % Q + (S / Q) * Q){I, L}[j] := Eq.symm <| ext_add_of_dvd_sq_right (le_trans (le_of_lt hij) hi) pq hq
+    _                           = S{I, L}[j]                     := by rw [mul_comm, add_comm, div_add_mod]
 
-def IsNuonSeq (a s : M) : Prop := ext a s 0 = 0 ∧ ∀ i < ‖a‖, ext a s (i + 1) = ext a s i + fbit a i
+variable {L A : M}
 
-def nuon (a n : M) : Prop := ∃ s, IsNuonSeq a s ∧ ext a s ‖a‖ = n
+def IsNuonIntvSeq (I L A start intv S : M) : Prop := ∀ i < intv, S{I, L}[i + 1] = S{I, L}[i] + fbit A (start + i)
+
+def NuonIntv (U I L A start intv nₛ nₑ : M) : Prop := ∃ S < U, IsNuonIntvSeq I L A start intv S ∧ S{I, L}[0] = nₛ ∧ S{I, L}[intv] = nₑ
+
+def IsNuonsSeq (U I L A cycle T : M) : Prop := ∀ l < cycle, NuonIntv U I L A (l * ‖I‖) ‖I‖ (T{I, L}[l]) (T{I, L}[l + 1])
+
+def NuonCycle (U I L A cycle n : M) : Prop := ∃ T < U, IsNuonsSeq U I L A cycle T ∧ T{I, L}[0] = 0 ∧ T{I, L}[cycle] = n
+
+def NuonPart (U I L A k n : M) : Prop := ∃ nₖ, NuonCycle U I L A (k / ‖I‖) nₖ ∧ NuonIntv U I L A (‖I‖ * k / ‖I‖) (k % ‖I‖) nₖ n
+
+/--/
+def Nuon₀ (K A n : M) : Prop := NuonIntv K A 0 ‖A‖ 0 n
+
+
+
+
+
+def Nuon₁ (A n : M) : Prop := NuonIntv A A 0 ‖A‖ 0 n
+
+
 
 end Nuon
 
